almost finished w/ IMM_S -> ARMv8 proof.

src/imm/imm_s.v
@@ -20,7 +20,6 @@ Remove Hints plus_n_O.
 Section IMM.
 
 Variable G : execution.
-Variable sc : relation actid.
 
 Notation "'E'" := G.(acts_set).
 Notation "'sb'" := G.(sb).
@@ -71,9 +70,6 @@ Notation "'Acqrel'" := (fun a => is_true (is_acqrel lab a)).
 Notation "'Acq/Rel'" := (fun a => is_true (is_ra lab a)).
 Notation "'Sc'" := (fun a => is_true (is_sc lab a)).
 
-
-
-
 (******************************************************************************)
 (** ** Derived relations  *)
 (******************************************************************************)
@@ -85,13 +81,13 @@ Definition scb := sb ∪ (sb \ same_loc) ⨾ hb ⨾ (sb \ same_loc) ∪
 Definition psc_base := ⦗ Sc ⦘ ⨾ (⦗ F ⦘ ⨾ hb)^? ⨾ scb ⨾ (hb ⨾ ⦗ F ⦘)^? ⨾ ⦗ Sc ⦘.
 Definition psc_f    := ⦗F∩₁Sc⦘ ⨾  hb ⨾ (eco ⨾ hb)^? ⨾ ⦗F∩₁Sc⦘.
 
-Definition ar := sc ∪ rfe ∪ ar_int.
+Definition ar sc := sc ∪ rfe ∪ ar_int.
 
 (******************************************************************************)
 (** ** Consistency  *)
 (******************************************************************************)
 
-Record wf_sc :=
+Record wf_sc sc :=
   { wf_scE : sc ≡ ⦗E⦘ ⨾ sc ⨾ ⦗E⦘ ;
     wf_scD : sc ≡ ⦗F∩₁Sc⦘ ⨾ sc ⨾ ⦗F∩₁Sc⦘ ;
     sc_trans : transitive sc ;
@@ -99,44 +95,48 @@ Record wf_sc :=
     sc_irr : irreflexive sc ;
   }.
 
-Definition acyc_ext := acyclic ar.
+Definition acyc_ext sc := acyclic (ar sc).
 
-Definition coh_sc := irreflexive (sc ⨾ hb ⨾ (eco ⨾ hb)^?).
+Definition coh_sc sc := irreflexive (sc ⨾ hb ⨾ (eco ⨾ hb)^?).
 
-Definition imm_consistent := 
-  ⟪ Wf_sc : wf_sc ⟫ /\
-  ⟪ Csc   : coh_sc ⟫ /\
+Definition imm_consistent sc := 
+  ⟪ Wf_sc : wf_sc sc ⟫ /\
+  ⟪ Csc   : coh_sc sc ⟫ /\
   ⟪ Comp  : complete G ⟫ /\
   ⟪ Cint  : coherence G ⟫ /\
-  ⟪ Cext  : acyc_ext ⟫ /\
+  ⟪ Cext  : acyc_ext sc ⟫ /\
   ⟪ Cat   : rmw_atomicity G ⟫.
 
-Definition imm_psc_consistent :=
-  ⟪ IC   : imm_consistent ⟫ /\
+Definition imm_psc_consistent sc :=
+  ⟪ IC   : imm_consistent sc ⟫ /\
   ⟪ Cpsc : acyclic (psc_f ∪ psc_base) ⟫.
 
-Implicit Type WF : Wf G.
-Implicit Type WF_SC : wf_sc.
-Implicit Type IMMCON : imm_consistent.
-Implicit Type CSC : coh_sc.
-Implicit Type COMP : complete G.
-Implicit Type COH : coherence G.
-Implicit Type ACYC_EXT : acyc_ext.
-Implicit Type AT : rmw_atomicity G.
+Hypothesis WF : Wf G.
+Hypothesis COH : coherence G.
+Hypothesis AT : rmw_atomicity G.
+
+Section SC.
+
+Variable sc : relation actid.
+
+Hypothesis WF_SC : wf_sc sc.
+Hypothesis IMMCON : imm_consistent sc.
+Hypothesis CSC : coh_sc sc.
+Hypothesis ACYC_EXT : acyc_ext sc.
 
 (******************************************************************************)
 (** ** Relations in graph *)
 (******************************************************************************)
 
-Lemma wf_pscE WF : psc ≡ ⦗E⦘ ⨾ psc ⨾ ⦗E⦘.
-Proof.
+Lemma wf_pscE : psc ≡ ⦗E⦘ ⨾ psc ⨾ ⦗E⦘.
+Proof using WF.
 split; [|basic_solver].
 unfold psc; rewrite (wf_hbE WF) at 1 2.
 basic_solver 42.
 Qed.
 
-Lemma wf_arE WF WF_SC : ar ≡ ⦗E⦘ ⨾ ar ⨾ ⦗E⦘.
-Proof.
+Lemma wf_arE : ar sc ≡ ⦗E⦘ ⨾ ar sc ⨾ ⦗E⦘.
+Proof using WF WF_SC.
 split; [|basic_solver].
 unfold ar.
 rewrite (wf_scE WF_SC), (wf_ar_intE WF), (wf_rfeE WF) at 1.
@@ -149,7 +149,7 @@ Qed.
 (******************************************************************************)
 
 Lemma wf_pscD : psc ≡ ⦗F∩₁Sc⦘ ⨾ psc ⨾ ⦗F∩₁Sc⦘.
-Proof.
+Proof using.
 split; [|basic_solver].
 unfold psc; basic_solver 42.
 Qed.
@@ -158,17 +158,17 @@ Qed.
 (** ** init *)
 (******************************************************************************)
 
-Lemma no_psc_to_init WF : psc ≡ psc ⨾  ⦗fun x => ~ is_init x⦘.
-Proof.
+Lemma no_psc_to_init : psc ≡ psc ⨾  ⦗fun x => ~ is_init x⦘.
+Proof using WF.
 split; [|basic_solver].
 rewrite wf_pscD at 1.
 generalize (read_or_fence_is_not_init WF).
 basic_solver 42.
 Qed.
 
-Lemma no_sc_to_init WF WF_SC :
+Lemma no_sc_to_init :
  sc ≡ sc ⨾  ⦗fun x => ~ is_init x⦘.
-Proof.
+Proof using WF WF_SC.
 split; [|basic_solver].
 rewrite wf_scD at 1; try done.
 generalize (read_or_fence_is_not_init WF).
@@ -179,9 +179,9 @@ Qed.
 (** ** more properties  *)
 (******************************************************************************)
 
-Lemma F_sc_ar_F_sc WF WF_SC ACYC_EXT:
-  ⦗F ∩₁ Sc⦘ ⨾ ar⁺ ⨾ ⦗F ∩₁ Sc⦘ ⊆ sc.
-Proof.
+Lemma F_sc_ar_F_sc :
+  ⦗F ∩₁ Sc⦘ ⨾ (ar sc)⁺ ⨾ ⦗F ∩₁ Sc⦘ ⊆ sc.
+Proof using WF WF_SC ACYC_EXT.
 rewrite wf_arE; try done.
 rewrite inclusion_ct_seq_eqv_l, inclusion_ct_seq_eqv_r.
 unfold ar.
@@ -194,16 +194,16 @@ intro; eapply ACYC_EXT; unfold ar; basic_solver.
 Qed.
 
 (* TODO: move to imm_s_ppo. *)
-Lemma rmw_in_ar_int WF : rmw ⊆ ar_int.
-Proof.
+Lemma rmw_in_ar_int : rmw ⊆ ar_int.
+Proof using WF.
   unfold imm_s_ppo.ar_int.
   rewrite WF.(rmw_in_ppo). eauto with hahn.
 Qed.
 
 (* TODO: move to imm_s_ppo. *)
-Lemma rfe_rmw_in_rfe_ar_int_ct WF : rfe ⨾ rmw ⊆ (rfe ∪ ar_int)⁺.
-Proof.
-  rewrite WF.(rmw_in_ar_int).
+Lemma rfe_rmw_in_rfe_ar_int_ct : rfe ⨾ rmw ⊆ (rfe ∪ ar_int)⁺.
+Proof using WF.
+  rewrite rmw_in_ar_int.
   arewrite (ar_int ⊆ rfe ∪ ar_int) at 1.
   arewrite (rfe ⊆ rfe ∪ ar_int) at 1.
   do 2 (rewrite ct_begin; rewrite rtE).
@@ -211,8 +211,8 @@ Proof.
 Qed.
 
 (* TODO: move to imm_s_ppo. *)
-Lemma ar_int_rfe_rfrmw_in_ar_int_rfe_ct WF : (rfe ∪ ar_int) ;; rf ;; rmw ⊆ (rfe ∪ ar_int)⁺.
-Proof.
+Lemma ar_int_rfe_rfrmw_in_ar_int_rfe_ct : (rfe ∪ ar_int) ;; rf ;; rmw ⊆ (rfe ∪ ar_int)⁺.
+Proof using WF.
   remember (rfe ∪ ar_int) as ax.
   assert (sb ;; sb ⊆ sb) as AA.
   { apply transitiveI. apply sb_trans. }
@@ -223,7 +223,7 @@ Proof.
   rewrite rfi_union_rfe.
   rewrite seq_union_l, seq_union_r.
   unionL.
-  2: { rewrite WF.(rfe_rmw_in_rfe_ar_int_ct).
+  2: { rewrite rfe_rmw_in_rfe_ar_int_ct.
        arewrite (ax ⊆ ax^?) at 1. subst ax. relsf. }
   subst ax.
   rewrite !seq_union_l.
@@ -255,29 +255,29 @@ Proof.
 Qed.
 
 (* TODO: move to imm_s_ppo. *)
-Lemma ar_int_rfe_rfrmw_rt_in_ar_int_rfe_ct WF :
+Lemma ar_int_rfe_rfrmw_rt_in_ar_int_rfe_ct :
   (rfe ∪ ar_int) ;; (rf ;; rmw)^* ⊆ (rfe ∪ ar_int)⁺.
-Proof.
+Proof using WF.
   apply rt_ind_left with (P:=fun r => (rfe ∪ ar_int) ⨾ r).
   { eauto with hahn. }
   { by rewrite seq_id_r, <- ct_step. }
-  ins. sin_rewrite WF.(ar_int_rfe_rfrmw_in_ar_int_rfe_ct).
+  ins. sin_rewrite ar_int_rfe_rfrmw_in_ar_int_rfe_ct.
   rewrite ct_end at 1. rewrite !seqA. rewrite H.
   relsf.
 Qed.
 
 (* TODO: move to imm_s_ppo. *)
-Lemma ar_int_rfe_ct_rfrmw_rt_in_ar_int_rfe_ct WF :
+Lemma ar_int_rfe_ct_rfrmw_rt_in_ar_int_rfe_ct :
   (rfe ∪ ar_int)⁺ ;; (rf ;; rmw)^* ⊆ (rfe ∪ ar_int)⁺.
-Proof.
+Proof using WF.
   rewrite ct_end at 1. rewrite !seqA. rewrite ar_int_rfe_rfrmw_rt_in_ar_int_rfe_ct; auto.
   relsf.
 Qed.
 
-Lemma sw_in_ar1 WF :
+Lemma sw_in_ar1 :
   sw ⊆ (<|F ∩₁ Rel|> ;; sb ∪ <|W ∩₁ Rel|> ;; (sb ∩ same_loc⨾ ⦗W⦘)^?) ⨾ 
   (rfe ∪ ar_int)⁺ ⨾ sb^? ∪ sb.
-Proof.
+Proof using WF.
   remember (rfe ∪ ar_int) as ax.
   unfold imm_s_hb.sw, imm_s_hb.release, imm_s_hb.rs.
   rewrite rt_rf_rmw.
@@ -290,7 +290,7 @@ Proof.
   { rewrite rtE at 1. rewrite seq_union_r. unionL.
     { basic_solver. }
     rewrite ct_begin, !seqA.
-    sin_rewrite WF.(rfe_rmw_in_rfe_ar_int_ct).
+    sin_rewrite rfe_rmw_in_rfe_ar_int_ct.
     arewrite ((rfi ⨾ rmw)＊ ⨾ (rfe ⨾ rmw ⨾ (rfi ⨾ rmw)＊)＊ ⊆ (rf ;; rmw)^*).
     { arewrite (rfi ⊆ rf). arewrite (rfe ⊆ rf).
       rewrite <- seqA, <- ct_begin. rewrite rt_of_ct. apply rt_rt. }
@@ -316,12 +316,12 @@ Proof.
   generalize (@sb_trans G). basic_solver 20.
 Qed.
 
-Lemma f_sc_hb_f_sc_in_rfe_ar_int WF :
+Lemma f_sc_hb_f_sc_in_rfe_ar_int :
   ⦗F ∩₁ Sc⦘ ⨾ hb ⨾ ⦗F ∩₁ Sc⦘ ⊆ (rfe ∪ ar_int)⁺.
-Proof.
+Proof using WF.
   unfold imm_s_hb.hb.
   rewrite (dom_l (wf_swD WF)).
-  rewrite (sw_in_ar1 WF).
+  rewrite sw_in_ar1.
   remember (rfe ∪ ar_int) as ax.
   rewrite seq_union_r.
   arewrite (⦗FW ∩₁ Rel⦘ ⨾ sb ⊆ sb).
@@ -369,75 +369,73 @@ Proof.
   basic_solver.
 Qed.
 
-Lemma f_sc_hb_f_sc_in_ar WF : 
-  ⦗F ∩₁ Sc⦘ ⨾ hb ⨾ ⦗F ∩₁ Sc⦘ ⊆ ar⁺.
-Proof.
-  rewrite WF.(f_sc_hb_f_sc_in_rfe_ar_int).
+Lemma f_sc_hb_f_sc_in_ar : 
+  ⦗F ∩₁ Sc⦘ ⨾ hb ⨾ ⦗F ∩₁ Sc⦘ ⊆ (ar sc)⁺.
+Proof using WF.
+  rewrite f_sc_hb_f_sc_in_rfe_ar_int.
   unfold ar. apply clos_trans_mori. eauto with hahn.
 Qed.
 
-Lemma f_sc_hb_f_sc_in_sc WF WF_SC ACYC_EXT: 
+Lemma f_sc_hb_f_sc_in_sc : 
   ⦗F ∩₁ Sc⦘ ⨾ hb ⨾ ⦗F ∩₁ Sc⦘ ⊆ sc.
-Proof.
+Proof using WF WF_SC ACYC_EXT.
 arewrite (⦗F ∩₁ Sc⦘ ⊆ ⦗F ∩₁ Sc⦘ ⨾ ⦗F ∩₁ Sc⦘) by basic_solver.
-sin_rewrite (f_sc_hb_f_sc_in_ar WF).
+sin_rewrite f_sc_hb_f_sc_in_ar.
 apply F_sc_ar_F_sc; done.
 Qed.
 
-Lemma wf_ar WF IMMCON : well_founded ar.
-Proof.
-  eapply wf_finite; auto.
+Lemma wf_ar : well_founded (ar sc).
+Proof using WF WF_SC IMMCON.
+  eapply wf_finite.
   { cdes IMMCON. apply Cext. }
   rewrite wf_arE; auto.
-  2: by apply IMMCON.
   apply doma_eqv.
 Qed.
 
-Lemma wf_ar_tc WF IMMCON : well_founded (ar⁺).
-Proof.
+Lemma wf_ar_tc : well_founded ((ar sc)⁺).
+Proof using WF WF_SC IMMCON.
   eapply wf_finite; auto.
   { cdes IMMCON. unfold acyclic. rewrite ct_of_ct.
     apply Cext. }
   rewrite wf_arE; auto.
-  2: by apply IMMCON.
   apply ct_doma. apply doma_eqv.
 Qed.
 
-Lemma ar_int_in_ar : ar_int ⊆ ar.
-Proof. unfold ar. basic_solver. Qed.
+Lemma ar_int_in_ar : ar_int ⊆ ar sc.
+Proof using. unfold ar. basic_solver. Qed.
 
-Lemma ppo_in_ar : ppo ⊆ ar.
-Proof.
+Lemma ppo_in_ar : ppo ⊆ ar sc.
+Proof using.
   etransitivity; [|by apply ar_int_in_ar].
   apply ppo_in_ar_int.
 Qed.
 
-Lemma bob_in_ar : bob ⊆ ar.
-Proof.
+Lemma bob_in_ar : bob ⊆ ar sc.
+Proof using.
   etransitivity; [|by apply ar_int_in_ar].
   apply bob_in_ar_int.
 Qed.
 
-Lemma detour_in_ar : detour ⊆ ar.
-Proof.
+Lemma detour_in_ar : detour ⊆ ar sc.
+Proof using.
   etransitivity; [|by apply ar_int_in_ar].
   apply detour_in_ar_int.
 Qed.
 
-Lemma rfe_in_ar : rfe ⊆ ar.
-Proof. unfold ar. basic_solver. Qed.
+Lemma rfe_in_ar : rfe ⊆ ar sc.
+Proof using. unfold ar. basic_solver. Qed.
 
-Lemma sc_in_ar : sc ⊆ ar.
-Proof. unfold ar. basic_solver. Qed.
+Lemma sc_in_ar : sc ⊆ ar sc.
+Proof using. unfold ar. basic_solver. Qed.
 
-Lemma w_ex_acq_sb_w_in_ar : ⦗W_ex_acq⦘ ⨾ sb ⨾ ⦗W⦘ ⊆ ar.
-Proof.
+Lemma w_ex_acq_sb_w_in_ar : ⦗W_ex_acq⦘ ⨾ sb ⨾ ⦗W⦘ ⊆ ar sc.
+Proof using.
   etransitivity; [|by apply ar_int_in_ar].
   apply w_ex_acq_sb_w_in_ar_int.
 Qed.
 
-Lemma coh_sc_alt WF WF_SC CSC COH : ⦗F∩₁Sc⦘ ⨾  hb ⨾ eco ⨾ hb ⨾ ⦗F∩₁Sc⦘ ⊆ sc.
-Proof.
+Lemma coh_sc_alt : ⦗F∩₁Sc⦘ ⨾  hb ⨾ eco ⨾ hb ⨾ ⦗F∩₁Sc⦘ ⊆ sc.
+Proof using WF WF_SC CSC COH.
 rewrite (dom_l (wf_hbE WF)) at 1.
 rewrite (dom_r (wf_hbE WF)) at 2.
 unfolder; ins; desf.
@@ -457,7 +455,7 @@ Proposition coh_helper_alt :
   hb ⨾ (sc ⨾ hb)^? ⨾ co ∪ hb ⨾ (sc ⨾ hb)^? ⨾ co ⨾ rfe ∪ 
   hb ⨾ (sc ⨾ hb)^? ⨾ fr ∪ hb ⨾ (sc ⨾ hb)^? ⨾ fr ⨾ rfe) -> 
   irreflexive (hb ⨾ (sc ⨾ hb)^? ⨾ eco^?).
-Proof.
+Proof using.
 unfold Execution_eco.eco; relsf.
 rewrite rfi_union_rfe; relsf.
 arewrite (rfi ⊆ sb); rewrite sb_in_hb; rewrite !crE; relsf.
@@ -468,11 +466,11 @@ all: try (unfolder in *; basic_solver 12).
 all: try (unfolder in *; basic_solver 16).
 Qed.
 
-Lemma init_co_w WF IMMCON
+Lemma init_co_w
       e e' (INIT : is_init e) (NINIT : ~ is_init e')
       (EE : E e') (WW : W e') (SL : same_loc e e') :
   co e e'.
-Proof.
+Proof using WF IMMCON.
   destruct (is_w_loc lab e' WW) as [l LOC].
   red in SL. rewrite LOC in SL.
   unfold is_init in INIT. unfold Events.loc in SL.
@@ -490,8 +488,8 @@ Proof.
   apply r_step. apply Execution_eco.co_in_eco; eauto.
 Qed.
 
-Lemma wf_rfrmw_irr WF IMMCON : irreflexive (rf ⨾ rmw).
-Proof.
+Lemma wf_rfrmw_irr : irreflexive (rf ⨾ rmw).
+Proof using WF IMMCON.
   arewrite (rmw ⊆ sb).
   { rewrite WF.(wf_rmwi). basic_solver. }
   rewrite Execution_eco.rf_in_eco.
@@ -499,22 +497,22 @@ Proof.
   red in Cint. generalize Cint. basic_solver 10.
 Qed.
 
-Lemma rfrmw_in_im_co WF IMMCON :
+Lemma rfrmw_in_im_co :
   rf ⨾ rmw ⊆ immediate co.
-Proof. 
+Proof using WF IMMCON. 
   cdes IMMCON.
   apply rf_rmw_in_coimm; auto using coherence_sc_per_loc.
 Qed.
 
-Lemma rfe_rmw_in_ar_ct WF : rfe ;; rmw ⊆ ar⁺.
-Proof.
+Lemma rfe_rmw_in_ar_ct : rfe ;; rmw ⊆ (ar sc)⁺.
+Proof using WF.
   rewrite <- ct_ct.
   rewrite rfe_in_ar, WF.(rmw_in_ppo), ppo_in_ar.
   eby rewrite <- ct_step.
 Qed.
 
-Lemma rfe_ppo_in_ar_ct : rfe ;; ppo ⊆ ar⁺.
-Proof.
+Lemma rfe_ppo_in_ar_ct : rfe ;; ppo ⊆ (ar sc)⁺.
+Proof using.
   rewrite <- ct_ct.
   rewrite rfe_in_ar, ppo_in_ar.
   eby rewrite <- ct_step.
@@ -522,7 +520,7 @@ Qed.
 
 (*
 Lemma rfe_Rex_sb_in_ar_ct : rfe ;; <|R_ex|> ;; sb ;; <|W|> ⊆ ar⁺.
-Proof.
+Proof using.
   arewrite (⦗R_ex⦘ ⨾ sb ⨾ ⦗W⦘ ⊆ ppo).
   2: by apply rfe_ppo_in_ar_ct.
   unfold imm_s_ppo.ppo. rewrite <- ct_step, !seq_union_l, !seq_union_r, !seqA.
@@ -533,7 +531,7 @@ Qed.
 
 (*
 Lemma rfe_rmw_sb_in_ar_ct WF : rfe ;; rmw ;; sb ;; <|W|> ⊆ ar⁺.
-Proof.
+Proof using.
   rewrite (dom_l WF.(wf_rmwD)), WF.(rmw_in_sb), !seqA.
   (* TODO: introduce a lemma *)
   arewrite (sb ;; sb ⊆ sb).
@@ -542,11 +540,11 @@ Proof.
 Qed.
 *)
 
-Lemma sb_release_rmw_in_fwbob WF
-      (SPL  : Execution_eco.sc_per_loc G)
-      (COMP : complete G) :
+Lemma sb_release_rmw_in_fwbob
+      (COMPL : complete G)
+      (SPL   : Execution_eco.sc_per_loc G) :
   sb^? ∩ release G ⨾ sb ∩ Events.same_loc lab ⨾ rmw ⊆ fwbob G.
-Proof.
+Proof using WF.
   rewrite (dom_r WF.(wf_rmwD)).
   rewrite WF.(rmw_in_sb_loc).
   sin_rewrite rewrite_trans.
@@ -577,51 +575,50 @@ Proof.
   unfold fwbob. eauto with hahn.
 Qed.
 
-Lemma no_ar_to_init WF IMMCON : ar ;; <|is_init|> ≡ ∅₂.
-Proof.
+Lemma no_ar_to_init : ar sc ;; <|is_init|> ≡ ∅₂.
+Proof using WF IMMCON.
   split; [|basic_solver].
   unfold ar.
   rewrite WF.(ar_int_in_sb). rewrite no_sb_to_init.
-  rewrite wf_scD; [|by apply IMMCON].
+  rewrite wf_scD with (sc:=sc); [|by apply IMMCON].
   rewrite WF.(wf_rfeD).
   rewrite seq_union_l. unionL; [|basic_solver].
   rewrite WF.(init_w). type_solver 10.
 Qed.
 
-Lemma no_ar_rfrmw_to_init WF IMMCON : (ar ∪ rf ⨾ rmw) ;; <|is_init|> ≡ ∅₂.
-Proof.
+Lemma no_ar_rfrmw_to_init : (ar sc ∪ rf ⨾ rmw) ;; <|is_init|> ≡ ∅₂.
+Proof using WF IMMCON.
   split; [|basic_solver].
   rewrite seq_union_l, seqA, no_ar_to_init; auto.
   rewrite WF.(rmw_in_sb). rewrite no_sb_to_init.
   basic_solver.
 Qed.
 
-Lemma wf_ar_rfrmwE WF IMMCON :
-  ar ∪ rf ;; rmw ≡ <|E|> ;; (ar ∪ rf ;; rmw) ;; <|E|>.
-Proof.
+Lemma wf_ar_rfrmwE :
+  ar sc ∪ rf ;; rmw ≡ <|E|> ;; (ar sc ∪ rf ;; rmw) ;; <|E|>.
+Proof using WF WF_SC IMMCON.
   rewrite wf_arE at 1; auto.
-  2: by apply IMMCON.
   rewrite (dom_l WF.(wf_rfE)) at 1.
   rewrite (dom_r WF.(wf_rmwE)) at 1.
   basic_solver 10.
 Qed.
 
-Lemma wf_ar_rfrmw_ctE WF IMMCON :
-  (ar ∪ rf ;; rmw)⁺ ≡ <|E|> ;; (ar ∪ rf ;; rmw)⁺ ;; <|E|>.
-Proof.
+Lemma wf_ar_rfrmw_ctE :
+  (ar sc ∪ rf ;; rmw)⁺ ≡ <|E|> ;; (ar sc ∪ rf ;; rmw)⁺ ;; <|E|>.
+Proof using WF WF_SC IMMCON.
   split; [|basic_solver].
   rewrite wf_ar_rfrmwE at 1; auto.
   rewrite inclusion_ct_seq_eqv_l.
     by rewrite inclusion_ct_seq_eqv_r.
 Qed.
 
-Lemma ar_ar_in_ar_ct : ar ;; ar ⊆ ar⁺.
-Proof.
-  rewrite ct_step with (r:=ar) at 1 2. apply ct_ct.
+Lemma ar_ar_in_ar_ct : ar sc ;; ar sc ⊆ (ar sc)⁺.
+Proof using.
+  rewrite ct_step with (r:=ar sc) at 1 2. apply ct_ct.
 Qed.
 
-Lemma rfe_n_same_tid WF IMMCON : rfe ∩ same_tid ⊆ ∅₂.
-Proof.
+Lemma rfe_n_same_tid : rfe ∩ same_tid ⊆ ∅₂.
+Proof using WF IMMCON.
   arewrite (rfe ∩ same_tid ⊆ rfe ∩ (<|E|> ;; same_tid ;; <|E|>)).
   { rewrite WF.(wf_rfeE) at 1. basic_solver. }
   arewrite (⦗E⦘ ⨾ same_tid ⨾ ⦗E⦘ ⊆ same_tid ∩ (⦗E⦘ ⨾ same_tid ⨾ ⦗E⦘)) by basic_solver.
@@ -647,14 +644,14 @@ Proof.
   basic_solver 10.
 Qed.
 
-Lemma ar_W_in_ar_int WF IMMCON : ar ;; <|W|> ⊆ ar_int.
-Proof.
-  unfold ar. erewrite wf_scD; [|by apply IMMCON].
+Lemma ar_W_in_ar_int : ar sc ;; <|W|> ⊆ ar_int.
+Proof using WF IMMCON.
+  unfold ar. erewrite wf_scD with (sc:=sc); [|by apply IMMCON].
   rewrite WF.(wf_rfeD). type_solver.
 Qed.
 
-Lemma C_EXT_helper2 WF: (psc ∪ rfe)⁺ ⊆ psc⁺ ∪ rfe.
-Proof.
+Lemma C_EXT_helper2 : (psc ∪ rfe)⁺ ⊆ psc⁺ ∪ rfe.
+Proof using WF.
 apply ct_ind_left with (P:= fun r => r).
 by eauto with hahn.
 by unionL; vauto.
@@ -666,17 +663,17 @@ rewrite (dom_r wf_pscD) at 1; rewrite (dom_l (wf_rfeD WF)); type_solver 12.
 rewrite (dom_r (wf_rfeD WF)) at 1; rewrite (dom_l (wf_rfeD WF)); type_solver 12.
 Qed.
 
-Lemma s_acyc_ext_helper WF
+Lemma s_acyc_ext_psc_helper
       (AC : acyclic (sb^? ⨾ psc ⨾ sb^? ∪ rfe ∪ ⦗R⦘ ⨾ ar_int⁺ ⨾ ⦗W⦘)) :
   acyclic (psc ∪ rfe ∪ ar_int).
-Proof.
+Proof using WF.
   generalize (@sb_trans G); intro SBT.
   red. apply acyclic_mon with (r:= ar_int ∪ (psc ∪ rfe)).
   2: by basic_solver 12.
   apply acyclic_union1.
   { rewrite (ar_int_in_sb WF). apply sb_acyclic. }
   { eapply acyclic_mon; [edone|basic_solver 12]. }
-  rewrite (C_EXT_helper2 WF); unionL.
+  rewrite C_EXT_helper2; unionL.
   arewrite (psc ⊆ sb^? ⨾ psc ⨾ sb^?) by basic_solver 12.
   relsf.
   rewrite (imm_s_ppo.ar_int_in_sb WF) at 1; relsf.
@@ -709,6 +706,51 @@ Proof.
   relsf.
   arewrite (rfe ⊆ (sb^? ⨾ psc ⨾ sb^? ∪ rfe ∪ ⦗R⦘ ⨾ ar_int⁺ ⨾ ⦗W⦘)＊) at 2.
   relsf; red; rels.
+Qed.
+
+End SC.
+
+Lemma s_acyc_ext_helper
+      (AC : acyclic (psc ∪ rfe ∪ ar_int)) :
+  exists sc, wf_sc sc /\ acyc_ext sc /\ coh_sc sc.
+Proof using WF.
+  set (ar' := psc ∪ rfe ∪ ar_int).
+  unfold acyc_ext.
+  exists (⦗ E ∩₁ F ∩₁ Sc ⦘ ⨾ tot_ext G.(acts) ar' ⨾ ⦗ E ∩₁ F ∩₁ Sc ⦘).
+  splits.
+  { constructor.
+    1,2: apply dom_helper_3; basic_solver.
+    { rewrite <- restr_relE; apply transitive_restr, tot_ext_trans. }
+    { unfolder; ins; desf.
+      cut (tot_ext (acts G) ar' a b \/ tot_ext (acts G) ar' b a).
+      { basic_solver 12. }
+      eapply tot_ext_total; desf; eauto. }
+    rewrite <- restr_relE.
+    apply irreflexive_restr. by apply tot_ext_irr. }
+  { unfold ar.
+    apply acyclic_mon with (r:= tot_ext (acts G) ar').
+    { apply trans_irr_acyclic.
+      { apply tot_ext_irr, AC. }
+      apply tot_ext_trans. }
+    apply inclusion_union_l; [apply inclusion_union_l|].
+    { basic_solver. }
+    all: subst ar'; rewrite <- tot_ext_extends; unfold ar; basic_solver. }
+  unfold coh_sc.
+  rotate 4.
+  arewrite (⦗E ∩₁ F ∩₁ Sc⦘ ⨾ hb ⨾ (eco ⨾ hb)^? ⨾ ⦗E ∩₁ F ∩₁ Sc⦘ ⊆ ar'⁺).
+  2: { arewrite (ar' ⊆ tot_ext (acts G) ar') at 2.
+       { apply tot_ext_extends. }
+       rewrite ct_step with (r:= tot_ext (acts G) ar') at 1.
+       rewrite ct_ct.
+       apply trans_irr_acyclic.
+       { apply tot_ext_irr, AC. }
+       apply tot_ext_trans. }
+  arewrite (⦗E ∩₁ F ∩₁ Sc⦘ ⊆ ⦗F ∩₁ Sc⦘) by basic_solver.
+  case_refl _. 
+  { erewrite f_sc_hb_f_sc_in_rfe_ar_int; eauto.
+    apply clos_trans_mori. subst ar'. eauto with hahn. }
+  rewrite !seqA. rewrite <- ct_step. subst ar'. 
+  unfold psc. eauto with hahn.
 Qed.
 
 End IMM.
